thir-elab/coq-extraction/Hacspec_chacha20.v
@@ -5,11 +5,15 @@ Open Scope Z_scope.
 Open Scope bool_scope.
 Open Scope hacspec_scope.
 
-Definition U8 := int8. (* Secret int  *)
-Definition U16 := int16. (* Secret int  *)
-Definition U32 := int32. (* Secret int  *)
-Definition U64 := int64. (* Secret int  *)
-Definition U128 := int128. (* Secret int  *)
+Definition int_xI {WS : WORDSIZE} (a : int) : int := MachineIntegers.add (MachineIntegers.mul a (repr 2)) MachineIntegers.one.
+Definition int_xO {WS : WORDSIZE} (a : int) : int := MachineIntegers.mul a (repr 2).
+Number Notation int Pos.of_num_int Pos.to_num_int (via positive mapping [[int_xI] => xI, [int_xO] => xO , [MachineIntegers.one] => xH]) : hacspec_scope.
+Notation "0" := (repr O).
+Notation U8 := int8. (* Secret int  *)
+Notation U16 := int16. (* Secret int  *)
+Notation U32 := int32. (* Secret int  *)
+Notation U64 := int64. (* Secret int  *)
+Notation U128 := int128. (* Secret int  *)
 
 Notation " x .[ a ]" := (array_index x a) (at level 40).
 Notation " x .[ i ]<- a" := (array_upd x i a) (at level 40).
@@ -18,6 +22,16 @@ Class Addition A := add : A -> A -> A.
 Notation "a .+ b" := (add a b).
 Instance array_add_inst {ws : WORDSIZE} {len: nat} : Addition (nseq (@int ws) len) := { add a b := a array_add b }.
 Instance int_add_inst {ws : WORDSIZE} : Addition (@int ws) := { add a b := MachineIntegers.add a b }.
+
+Class Subtraction A := sub : A -> A -> A.
+Notation "a .- b" := (sub a b).
+Instance array_sub_inst {ws : WORDSIZE} {len: nat} : Subtraction (nseq (@int ws) len) := { sub := array_join_map MachineIntegers.sub }.
+Instance int_sub_inst {ws : WORDSIZE} : Subtraction (@int ws) := { sub a b := MachineIntegers.sub a b }.
+
+Class Multiplication A := mul : A -> A -> A.
+Notation "a .* b" := (mul a b).
+Instance array_mul_inst {ws : WORDSIZE} {len: nat} : Multiplication (nseq (@int ws) len) := { mul a b := a array_mul b }.
+Instance int_mul_inst {ws : WORDSIZE} : Multiplication (@int ws) := { mul a b := MachineIntegers.mul a b }.
 
 Class Xor A := xor : A -> A -> A.
 Notation "a .^ b" := (xor a b).
@@ -31,6 +45,8 @@ Class array_or_seq A len :=
 
 Arguments as_seq {_} {_} array_or_seq.
 Arguments as_nseq {_} {_} array_or_seq.
+Coercion as_seq : array_or_seq >-> seq.
+Coercion as_nseq : array_or_seq >-> nseq.
 
 Instance nseq_array_or_seq {A len} (a : nseq A len) : array_or_seq A len :=
 { as_seq := array_to_seq a ; as_nseq := a ; }.
@@ -45,10 +61,10 @@ array_update (a := A) (len := len) s start (as_seq start_a).
 
 Definition to_le_U32s {A l} := array_to_le_uint32s (A := A) (l := l).
 Axiom to_le_bytes : forall {ws : WORDSIZE} {len}, nseq (@int ws) len -> seq int8.
-Definition from_seq {A : Type}  `{Default A} {len} (s : seq A) : nseq A len := array_from_seq _ s.
+Definition from_seq {A : Type}  `{Default A} {len slen} (s : array_or_seq A slen) : nseq A len := array_from_seq _ (as_seq s).
 
 Notation Seq := seq.
-Notation len := length.
+Notation len := (fun s => seq_len s : int32).
 
 Notation slice := array_slice.
 Notation new_seq := seq_new.
@@ -66,6 +82,29 @@ seq_set_chunk s chunk_len chunk_num (as_seq chunk).
 Definition set_exact_chunk {a} `{H : Default a} {len} := @set_chunk a H len.
 Notation get_remainder_chunk := seq_get_remainder_chunk.
 Notation "a <> b" := (negb (eqb a b)).
+
+Notation from_secret_literal := nat_mod_from_secret_literal.
+Definition pow2 {m} (x : @int WORDSIZE32) := nat_mod_pow2 m (unsigned x).
+Instance nat_mod_addition {n} : Addition (nat_mod n) := { add a b := a +% b }.
+Instance nat_mod_subtraction {n} : Subtraction (nat_mod n) := { sub a b := a -% b }.
+Instance nat_mod_multiplication {n} : Multiplication (nat_mod n) := { mul a b := a *% b }.
+Definition from_slice {a: Type} `{Default a} {len slen} (x : array_or_seq a slen) := array_from_slice default len (as_seq x).
+Notation zero := nat_mod_zero.
+Notation to_byte_seq_le := nat_mod_to_byte_seq_le.
+Notation U128_to_le_bytes := u128_to_le_bytes.
+Notation from_byte_seq_le := nat_mod_from_byte_seq_le.
+Definition from_literal {m} := nat_mod_from_literal m.
+Notation inv := nat_mod_inv.
+Notation update_start := array_update_start.
+Notation pow := nat_mod_pow_self.
+Notation bit := nat_mod_bit.
+
+Definition int_to_int {ws1 ws2} (i : @int ws1) : @int ws2 := repr (unsigned i).
+Coercion int_to_int : int >-> int.
+Notation push := seq_push.
+Notation Build_secret := secret.
+Notation "a -× b" :=
+(prod a b) (at level 80, right associativity) : hacspec_scope.
 
 
 (*Not implemented yet? todo(item)*)
@@ -85,88 +124,88 @@ Notation ChaChaIV := (nseq int8 12).
 Notation ChaChaKey := (nseq int8 32).
 
 Definition chacha20_line (a : int32) (b : int32) (d : int32) (s : int32) (m : State) : State :=
-  let state : State := m in
-  let state : State := state.[a]<-((state.[a]).+(state.[b])) in
-  let state : State := state.[d]<-((state.[d]).^(state.[a])) in
+  let state := m : State in
+  let state := state.[a]<-((state.[a]).+(state.[b])) : State in
+  let state := state.[d]<-((state.[d]).^(state.[a])) : State in
   state.[d]<-(rol (state.[d]) s).
 
 Definition chacha20_quarter_round (a : int32) (b : int32) (c : int32) (d : int32) (state : State) : State :=
-  let state : State := chacha20_line a b d 16 state in
-  let state : State := chacha20_line c d b 12 state in
-  let state : State := chacha20_line a b d 8 state in
+  let state := chacha20_line a b d 16 state : State in
+  let state := chacha20_line c d b 12 state : State in
+  let state := chacha20_line a b d 8 state : State in
   chacha20_line c d b 7 state.
 
 Definition chacha20_double_round (state : State) : State :=
-  let state : State := chacha20_quarter_round 0 4 8 12 state in
-  let state : State := chacha20_quarter_round 1 5 9 13 state in
-  let state : State := chacha20_quarter_round 2 6 10 14 state in
-  let state : State := chacha20_quarter_round 3 7 11 15 state in
-  let state : State := chacha20_quarter_round 0 5 10 15 state in
-  let state : State := chacha20_quarter_round 1 6 11 12 state in
-  let state : State := chacha20_quarter_round 2 7 8 13 state in
+  let state := chacha20_quarter_round 0 4 8 12 state : State in
+  let state := chacha20_quarter_round 1 5 9 13 state : State in
+  let state := chacha20_quarter_round 2 6 10 14 state : State in
+  let state := chacha20_quarter_round 3 7 11 15 state : State in
+  let state := chacha20_quarter_round 0 5 10 15 state : State in
+  let state := chacha20_quarter_round 1 6 11 12 state : State in
+  let state := chacha20_quarter_round 2 7 8 13 state : State in
   chacha20_quarter_round 3 4 9 14 state.
 
 Definition chacha20_rounds (state : State) : State :=
-  let st : State := state in
+  let st := state : State in
   foldi 0 10 (fun _i st =>
     chacha20_double_round st) st.
 
 Definition chacha20_core (ctr : U32) (st0 : State) : State :=
-  let state : State := st0 in
-  let state : State := state.[12]<-((state.[12]).+ctr) in
-  let k : State := chacha20_rounds state in
+  let state := st0 : State in
+  let state := state.[12]<-((state.[12]).+ctr) : State in
+  let k := chacha20_rounds state : State in
   k.+state.
 
 Definition chacha20_constants_init : Constants :=
-  let constants : Constants := new in
-  let constants : Constants := constants.[0]<-(secret 1634760805) in
-  let constants : Constants := constants.[1]<-(secret 857760878) in
-  let constants : Constants := constants.[2]<-(secret 2036477234) in
-  constants.[3]<-(secret 1797285236).
+  let constants := new : Constants in
+  let constants := constants.[0]<-(Build_secret 1634760805) : Constants in
+  let constants := constants.[1]<-(Build_secret 857760878) : Constants in
+  let constants := constants.[2]<-(Build_secret 2036477234) : Constants in
+  constants.[3]<-(Build_secret 1797285236).
 
 Definition chacha20_init (key : ChaChaKey) (iv : ChaChaIV) (ctr : U32) : State :=
-  let st : State := new in
-  let st : State := update st 0 chacha20_constants_init in
-  let st : State := update st 4 (to_le_U32s key) in
-  let st : State := st.[12]<-ctr in
+  let st := new : State in
+  let st := update st 0 chacha20_constants_init : State in
+  let st := update st 4 (to_le_U32s key) : State in
+  let st := st.[12]<-ctr : State in
   update st 13 (to_le_U32s iv).
 
 Definition chacha20_key_block (state : State) : Block :=
-  let state : State := chacha20_core (secret 0) state in
+  let state := chacha20_core (Build_secret 0) state : State in
   from_seq (to_le_bytes state).
 
 Definition chacha20_key_block0 (key : ChaChaKey) (iv : ChaChaIV) : Block :=
-  let state : State := chacha20_init key iv (secret 0) in
+  let state := chacha20_init key iv (Build_secret 0) : State in
   chacha20_key_block state.
 
 Definition chacha20_encrypt_block (st0 : State) (ctr : U32) (plain : Block) : Block :=
-  let st : State := chacha20_core ctr st0 in
-  let pl : State := from_seq (to_le_U32s plain) in
-  let st : State := pl.^st in
+  let st := chacha20_core ctr st0 : State in
+  let pl := from_seq (to_le_U32s plain) : State in
+  let st := pl.^st : State in
   from_seq (to_le_bytes st).
 
 Definition chacha20_encrypt_last (st0 : State) (ctr : U32) (plain : Seq U8) : Seq U8 :=
-  let b : Block := new in
-  let b : Block := update b 0 plain in
-  let b : Block := chacha20_encrypt_block st0 ctr b in
+  let b := new : Block in
+  let b := update b 0 plain : Block in
+  let b := chacha20_encrypt_block st0 ctr b : Block in
   slice b 0 (len plain).
 
 Definition chacha20_update (st0 : State) (m : Seq U8) : Seq U8 :=
-  let blocks_out : Seq U8 := new_seq (len m) in
-  let n_blocks : int32 := num_exact_chunks m 64 in
-  let blocks_out : Seq U8 := foldi 0 n_blocks (fun i blocks_out =>
-      let msg_block : Seq U8 := get_exact_chunk m 64 i in
-      let b : Block := chacha20_encrypt_block st0 (secret i) (from_seq msg_block) in
-      set_exact_chunk blocks_out 64 i b) blocks_out in
-  let last_block : Seq U8 := get_remainder_chunk m 64 in
+  let blocks_out := new_seq (len m) : Seq U8 in
+  let n_blocks := num_exact_chunks m 64 : int32 in
+  let blocks_out := foldi 0 n_blocks (fun i blocks_out =>
+      let msg_block := get_exact_chunk m 64 i : Seq U8 in
+      let b := chacha20_encrypt_block st0 (Build_secret i) (from_seq msg_block) : Block in
+      set_exact_chunk blocks_out 64 i b) blocks_out : Seq U8 in
+  let last_block := get_remainder_chunk m 64 : Seq U8 in
   if
     (len last_block)<>0
   then
-    let b : Seq U8 := chacha20_encrypt_last st0 (secret n_blocks) last_block in
+    let b := chacha20_encrypt_last st0 (Build_secret n_blocks) last_block : Seq U8 in
     set_chunk blocks_out 64 n_blocks b
   else
     blocks_out.
 
 Definition chacha20 (key : ChaChaKey) (iv : ChaChaIV) (ctr : int32) (m : Seq U8) : Seq U8 :=
-  let state : State := chacha20_init key iv (secret ctr) in
+  let state := chacha20_init key iv (Build_secret ctr) : State in
   chacha20_update state m.
