thir-elab/coq-extraction/Hacspec_poly1305.v
@@ -5,11 +5,15 @@ Open Scope Z_scope.
 Open Scope bool_scope.
 Open Scope hacspec_scope.
 
-Definition U8 := int8. (* Secret int  *)
-Definition U16 := int16. (* Secret int  *)
-Definition U32 := int32. (* Secret int  *)
-Definition U64 := int64. (* Secret int  *)
-Definition U128 := int128. (* Secret int  *)
+Definition int_xI {WS : WORDSIZE} (a : int) : int := MachineIntegers.add (MachineIntegers.mul a (repr 2)) MachineIntegers.one.
+Definition int_xO {WS : WORDSIZE} (a : int) : int := MachineIntegers.mul a (repr 2).
+Number Notation int Pos.of_num_int Pos.to_num_int (via positive mapping [[int_xI] => xI, [int_xO] => xO , [MachineIntegers.one] => xH]) : hacspec_scope.
+Notation "0" := (repr O).
+Notation U8 := int8. (* Secret int  *)
+Notation U16 := int16. (* Secret int  *)
+Notation U32 := int32. (* Secret int  *)
+Notation U64 := int64. (* Secret int  *)
+Notation U128 := int128. (* Secret int  *)
 
 Notation " x .[ a ]" := (array_index x a) (at level 40).
 Notation " x .[ i ]<- a" := (array_upd x i a) (at level 40).
@@ -18,6 +22,11 @@ Class Addition A := add : A -> A -> A.
 Notation "a .+ b" := (add a b).
 Instance array_add_inst {ws : WORDSIZE} {len: nat} : Addition (nseq (@int ws) len) := { add a b := a array_add b }.
 Instance int_add_inst {ws : WORDSIZE} : Addition (@int ws) := { add a b := MachineIntegers.add a b }.
+
+Class Subtraction A := sub : A -> A -> A.
+Notation "a .- b" := (sub a b).
+Instance array_sub_inst {ws : WORDSIZE} {len: nat} : Subtraction (nseq (@int ws) len) := { sub := array_join_map MachineIntegers.sub }.
+Instance int_sub_inst {ws : WORDSIZE} : Subtraction (@int ws) := { sub a b := MachineIntegers.sub a b }.
 
 Class Multiplication A := mul : A -> A -> A.
 Notation "a .* b" := (mul a b).
@@ -55,7 +64,7 @@ Axiom to_le_bytes : forall {ws : WORDSIZE} {len}, nseq (@int ws) len -> seq int8
 Definition from_seq {A : Type}  `{Default A} {len slen} (s : array_or_seq A slen) : nseq A len := array_from_seq _ (as_seq s).
 
 Notation Seq := seq.
-Notation len := length.
+Notation len := (fun s => seq_len s : int32).
 
 Notation slice := array_slice.
 Notation new_seq := seq_new.
@@ -75,13 +84,27 @@ Notation get_remainder_chunk := seq_get_remainder_chunk.
 Notation "a <> b" := (negb (eqb a b)).
 
 Notation from_secret_literal := nat_mod_from_secret_literal.
-Definition pow2 {m} := nat_mod_pow2 m.
+Definition pow2 {m} (x : @int WORDSIZE32) := nat_mod_pow2 m (unsigned x).
 Instance nat_mod_addition {n} : Addition (nat_mod n) := { add a b := a +% b }.
+Instance nat_mod_subtraction {n} : Subtraction (nat_mod n) := { sub a b := a -% b }.
 Instance nat_mod_multiplication {n} : Multiplication (nat_mod n) := { mul a b := a *% b }.
 Definition from_slice {a: Type} `{Default a} {len slen} (x : array_or_seq a slen) := array_from_slice default len (as_seq x).
 Notation zero := nat_mod_zero.
 Notation to_byte_seq_le := nat_mod_to_byte_seq_le.
 Notation U128_to_le_bytes := u128_to_le_bytes.
+Notation from_byte_seq_le := nat_mod_from_byte_seq_le.
+Definition from_literal {m} := nat_mod_from_literal m.
+Notation inv := nat_mod_inv.
+Notation update_start := array_update_start.
+Notation pow := nat_mod_pow_self.
+Notation bit := nat_mod_bit.
+
+Definition int_to_int {ws1 ws2} (i : @int ws1) : @int ws2 := repr (unsigned i).
+Coercion int_to_int : int >-> int.
+Notation push := seq_push.
+Notation Build_secret := secret.
+Notation "a -× b" :=
+(prod a b) (at level 80, right associativity) : hacspec_scope.
 
 
 (*Not implemented yet? todo(item)*)
@@ -106,11 +129,11 @@ Notation BlockIndex := (int32).
 Notation FieldCanvas := (nseq int8 131).
 Notation FieldElement := (nat_mod 0x03fffffffffffffffffffffffffffffffb).
 
-Notation PolyState := (FieldElement '× FieldElement '× PolyKey).
+Notation PolyState := ((FieldElement '× FieldElement '× PolyKey)).
 
 Definition poly1305_encode_r (b : PolyBlock) : FieldElement :=
   let n := uint128_from_le_bytes (from_seq b) : U128 in
-  let n := n.&(secret 21267647620597763993911028882763415551) : U128 in
+  let n := n.&(Build_secret 21267647620597763993911028882763415551) : U128 in
   from_secret_literal n.
 
 Definition poly1305_encode_block (b : PolyBlock) : FieldElement :=
@@ -121,46 +144,46 @@ Definition poly1305_encode_block (b : PolyBlock) : FieldElement :=
 Definition poly1305_encode_last (pad_len : int32) (b : Seq U8) : FieldElement :=
   let n := uint128_from_le_bytes (from_slice b 0 (len b)) : U128 in
   let f := from_secret_literal n : FieldElement in
-  f.+(pow2 (8*pad_len)).
+  f.+(pow2 (8.*pad_len)).
 
-Definition poly1305_init (k : PolyKey) : FieldElement '× FieldElement '× PolyKey :=
+Definition poly1305_init (k : PolyKey) : (FieldElement '× FieldElement '× PolyKey) :=
   let r := poly1305_encode_r (from_slice k 0 16) : FieldElement in
   (zero,r,k).
 
-Definition poly1305_update_block (b : PolyBlock) (st : FieldElement '× FieldElement '× PolyKey) : FieldElement '× FieldElement '× PolyKey :=
-  let '(acc,r,k) := st : FieldElement '× FieldElement '× PolyKey in
+Definition poly1305_update_block (b : PolyBlock) (st : (FieldElement '× FieldElement '× PolyKey)) : (FieldElement '× FieldElement '× PolyKey) :=
+  let '(acc,r,k) := st : (FieldElement '× FieldElement '× PolyKey) in
   (((poly1305_encode_block b).+acc).*r,r,k).
 
-Definition poly1305_update_blocks (m : Seq U8) (st : FieldElement '× FieldElement '× PolyKey) : FieldElement '× FieldElement '× PolyKey :=
-  let st := st : FieldElement '× FieldElement '× PolyKey in
+Definition poly1305_update_blocks (m : Seq U8) (st : (FieldElement '× FieldElement '× PolyKey)) : (FieldElement '× FieldElement '× PolyKey) :=
+  let st := st : (FieldElement '× FieldElement '× PolyKey) in
   let n_blocks := (len m)/BLOCKSIZE : int32 in
   foldi 0 n_blocks (fun i st =>
     let block := from_seq (get_exact_chunk m BLOCKSIZE i) : PolyBlock in
     poly1305_update_block block st) st.
 
-Definition poly1305_update_last (pad_len : int32) (b : Seq U8) (st : FieldElement '× FieldElement '× PolyKey) : FieldElement '× FieldElement '× PolyKey :=
-  let st := st : FieldElement '× FieldElement '× PolyKey in
+Definition poly1305_update_last (pad_len : int32) (b : Seq U8) (st : (FieldElement '× FieldElement '× PolyKey)) : (FieldElement '× FieldElement '× PolyKey) :=
+  let st := st : (FieldElement '× FieldElement '× PolyKey) in
   if
     (len b)<>0
   then
-    let '(acc,r,k) := st : FieldElement '× FieldElement '× PolyKey in
+    let '(acc,r,k) := st : (FieldElement '× FieldElement '× PolyKey) in
     (((poly1305_encode_last pad_len b).+acc).*r,r,k)
   else
     st.
 
-Definition poly1305_update (m : Seq U8) (st : FieldElement '× FieldElement '× PolyKey) : FieldElement '× FieldElement '× PolyKey :=
-  let st := poly1305_update_blocks m st : FieldElement '× FieldElement '× PolyKey in
+Definition poly1305_update (m : Seq U8) (st : (FieldElement '× FieldElement '× PolyKey)) : (FieldElement '× FieldElement '× PolyKey) :=
+  let st := poly1305_update_blocks m st : (FieldElement '× FieldElement '× PolyKey) in
   let last := get_remainder_chunk m BLOCKSIZE : Seq U8 in
   poly1305_update_last (len last) last st.
 
-Definition poly1305_finish (st : FieldElement '× FieldElement '× PolyKey) : Poly1305Tag :=
-  let '(acc,_,k) := st : FieldElement '× FieldElement '× PolyKey in
+Definition poly1305_finish (st : (FieldElement '× FieldElement '× PolyKey)) : Poly1305Tag :=
+  let '(acc,_,k) := st : (FieldElement '× FieldElement '× PolyKey) in
   let n := uint128_from_le_bytes (from_slice k 16 16) : U128 in
   let aby := to_byte_seq_le acc : Seq U8 in
   let a := uint128_from_le_bytes (from_slice aby 0 16) : U128 in
   from_seq (U128_to_le_bytes (a.+n)).
 
 Definition poly1305 (m : Seq U8) (key : PolyKey) : Poly1305Tag :=
-  let st := poly1305_init key : FieldElement '× FieldElement '× PolyKey in
-  let st := poly1305_update m st : FieldElement '× FieldElement '× PolyKey in
+  let st := poly1305_init key : (FieldElement '× FieldElement '× PolyKey) in
+  let st := poly1305_update m st : (FieldElement '× FieldElement '× PolyKey) in
   poly1305_finish st.
